mwes

Qsort/Monadic/MWEs.lean
@@ -4,6 +4,8 @@ open Std.Do
 
 set_option mvcgen.warning false
 
+--- --- --- ---
+
 namespace AssumptionFail
 
 axiom G (lt : Nat) : Id Unit
@@ -21,16 +23,16 @@ theorem qpartition_sorted (h : P) :
    ⦃⌜True⌝⦄ F ⦃⇓ _ => ⌜0 < 1⌝⦄ := by
   unfold F
   mvcgen
-  -- FIXME `mvcgen` should have handled this; is the `autoParam` interfering here?
+  -- FIXME (1) mvcgen should have handled this; is the `autoParam` interfering here?
   case h => assumption
 
 end AssumptionFail
 
+--- --- --- ---
+
 namespace MakeGoalPure
 
 abbrev SM := StateM Nat
-
-abbrev ps := PostShape.arg Nat PostShape.pure
 
 axiom P : Nat → Prop
 axiom P' : Nat → Prop
@@ -56,7 +58,6 @@ axiom G_spec : ⦃⌜True⌝⦄ G ⦃⇓ _ => ⌜P #n⌝ ∧ ⌜P' #n⌝⦄
 @[spec]
 axiom H_spec : ⦃⌜Q #n⌝⦄ H ⦃⇓ _ => R⦄
 
--- set_option pp.proofs true in
 theorem F_spec :
    ⦃⌜True⌝⦄
    F
@@ -64,7 +65,7 @@ theorem F_spec :
   unfold F
   mvcgen
 
-  -- ideally, mvcgen would do these four steps automatically for us
+  -- FIXME (2) ideally, mvcgen would do these four steps automatically for us
   mintro ∀_
   mframe
   mpure_intro
@@ -95,3 +96,148 @@ theorem F_spec' :
   apply hPQ <;> assumption
 
 end MakeGoalPure
+
+--- --- --- ---
+
+namespace LoopStuff
+
+abbrev SM := StateM (Array Nat)
+
+abbrev gns : SVal ((Array Nat)::[]) (Array Nat) := fun s => SVal.pure s
+
+noncomputable def setZero : StateM (Array Nat) Unit := do
+  let mut i := 0
+  let len := (← get).size
+  for _ in [0:len] do
+    let ns ← get
+    if h : i < ns.size then
+      modify fun _ => ns.set i 0 h
+    i := i + 1
+
+theorem setZero_spec :
+   ⦃⌜#gns = ns⌝⦄
+   setZero
+   -- FIXME (3.1) why parens needed around #gns?
+   ⦃⇓ _ => ⌜(#gns).size = ns.size⌝ ∧ ⌜∀ i, (h : i < (#gns).size) → (#gns)[i]'h = 0⌝⦄ := by
+  unfold setZero
+  mvcgen
+
+  case inv =>
+    exact ⇓ (i, sp) =>
+      -- FIXME (3.2) it would be very convenient to be able to name each of these
+      -- components, and have mvcgen automatically call `rcases h with ...` to
+      -- destruct it into separate hypotheses (using these names) in every
+      -- subsequent goal. Then we wouldn't have to do it ourselves.
+      ⌜(#gns).size = ns.size⌝ ∧
+      ⌜ i = sp.rpref.length ⌝ ∧
+      ⌜∀ j, (j < i) → (h : j < (#gns).size) → (#gns)[j]'h = 0⌝
+
+  -- FIXME (3.3) why did `i` get renamed to `b`?
+  . mvcgen_aux
+    rcases h with ⟨hs, hi, hz⟩ -- FIXME (3.2)
+
+    simp only [← hs]
+    simp only [Array.size_set]
+    and_intros
+    . trivial
+    . simp
+      exact hi
+    intros j hj hjs
+    if j < b then
+      rw [Array.getElem_set_ne]
+      apply hz
+      assumption
+      omega
+      omega
+    else
+      have : j = b := by omega
+      subst this
+      apply Array.getElem_set_self
+
+  . mvcgen_aux
+    rcases h with ⟨hs, hi, hz⟩ -- FIXME see (3.2)
+
+    -- FIXME (3.4) this should be automated, somehow?
+    -- Perhaps by annotating the spec's precondition `⌜#gns = ns⌝` in some way
+    next hns _ _ =>
+    have hns := hns.symm
+    subst hns
+    clear hns
+
+    -- FIXME (3.5) this property should be provided to us by `Spec.forIn_range`?
+    have hrng_dec_sz : (rpref.reverse ++ x :: suff).length = len := by
+      rw [← h]
+      simp only [List.length_range', Nat.sub_zero, Nat.add_one_sub_one, Nat.div_one]
+    rw [List.length_append, List.length_reverse, List.length_cons] at hrng_dec_sz
+
+    subst hi
+    have : rpref.length < ns.size := by omega
+    rw [hs] at *
+    contradiction
+
+  . mvcgen_aux
+
+    subst h
+    and_intros
+    rfl
+    rfl
+    omega
+
+  . mvcgen_aux
+    -- FIXME (3.6) these simplifications are specific to the use of `Specs.forin_range`,
+    -- and should probably be automatically applied whenever that spec is used
+    simp only [List.length_reverse, List.length_range'] at h
+    simp only [Nat.add_one_sub_one, Nat.div_one] at h
+
+    -- FIXME see (3.4)
+    next hns _ _ =>
+    have hns := hns.symm
+    subst hns
+    clear hns
+
+    rcases h with ⟨hs, hi, hz⟩ -- FIXME see (2)
+
+    simp only [Nat.sub_zero] at hi
+    subst hi
+    rw [← hs]
+    and_intros
+    rfl
+    intros i hi'
+    apply hz
+    omega
+    omega
+
+end LoopStuff
+
+--- --- --- ---
+
+namespace NeedStateLVar
+
+abbrev SM := StateM (Array Nat)
+
+abbrev gns : SVal ((Array Nat)::[]) (Array Nat) := fun s => SVal.pure s
+
+noncomputable def setZeroHead : StateM (Array Nat) Unit := do
+  modify fun _ => #[0, 1, 2, 3, 4, 5]
+
+macro "mvcgen_aux" : tactic => do
+  `(tactic|
+    (repeat mintro ∀_
+     try mframe
+     mpure_intro
+     simp only [SPred.and_cons, SVal.curry_cons, SVal.curry_nil, SVal.uncurry_cons, SVal.uncurry_nil, SPred.and_nil] at *))
+
+theorem setZeroHead_spec :
+   ⦃⌜True⌝⦄
+   setZeroHead
+   ⦃⇓ _ => ⌜∃ ns', (#gns).toList = 0 :: ns'⌝⦄ := by
+  unfold setZeroHead
+  mvcgen
+
+  . -- FIXME (4) here, we would want mvcgen to have assigned some let variable
+    -- `s := #[0, 1, 2, 3, 4, 5]` so that we can use `s.tail` below instead of
+    -- having to rewrite part of the state that was set with `modify`
+    mvcgen_aux
+    exists [1, 2, 3, 4, 5]
+
+end NeedStateLVar
